Transitivity

Auto/Embedding/LamThm.lean
@@ -16,7 +16,7 @@ def Eq.symm.WF (wf : LamWF ltv ⟨lctx, .app (.app (.base (.eq n)) a) b, .base .
 theorem Eq.symm (lval : LamValuation)
   {lctxTy : Nat → LamSort} {lctxTerm : ∀ n, (lctxTy n).interp lval.ilVal.tyVal}
   (wf : LamWF lval.ilVal.toLamTyVal ⟨lctxTy, .app (.app (.base (.eq n)) a) b, .base .prop⟩)
-  (_ : GLift.down (LamWF.interp lval lctxTy lctxTerm wf)) :
+  (H : GLift.down (LamWF.interp lval lctxTy lctxTerm wf)) :
   GLift.down (LamWF.interp lval lctxTy lctxTerm (Eq.symm.WF wf)) :=
   match wf with
   | .ofApp argTy wfFn wfB =>
@@ -24,11 +24,70 @@ theorem Eq.symm (lval : LamValuation)
     | .ofApp argTy' wfEq wfA =>
       match wfEq with
       | .ofBase HB => by
-        cases HB; case ofEq H =>
-        dsimp [symm.WF, LamWF.interp, LamBaseWF.interp];
-        dsimp [symm.WF, LamWF.interp, LamBaseWF.interp] at H;
+        cases HB; case ofEq =>
         have H' := EqLift.down _ _ _ H
         apply EqLift.up
         exact (_root_.Eq.symm H')
+
+def Eq.trans.WF
+  (wf₁ : LamWF ltv ⟨lctx, .app (.app (.base (.eq m)) a) b, .base .prop⟩)
+  (wf₂ : LamWF ltv ⟨lctx, .app (.app (.base (.eq n)) b) c, .base .prop⟩)
+  : LamWF ltv ⟨lctx, .app (.app (.base (.eq n)) a) c, .base .prop⟩ :=
+  match wf₁ with
+  | .ofApp argTy₁ wfFn₁ wfB₁ =>
+    match wfFn₁ with
+    | .ofApp argTy₁' wfEq₁ wfA =>
+      match wfEq₁ with
+      | .ofBase HB₁ =>
+        match HB₁ with
+        | .ofEq m =>
+          match wf₂ with
+          | .ofApp argTy₂ wfFn₂ wfC =>
+            match wfFn₂ with
+            | .ofApp argTy₂' wfEq₂ wfB₂ =>
+              match wfEq₂ with
+              | .ofBase HB₂ =>
+                match HB₂ with
+                | .ofEq n =>
+                  let heq : LamTyVal.eqLamVal ltv m = LamTyVal.eqLamVal ltv n :=
+                    (LamWF.unique ltv wfB₁ wfB₂).left
+                  .ofApp _ (.ofApp _ (.ofBase (.ofEq n)) (heq ▸ wfA)) wfC
+
+theorem Eq.trans (lval : LamValuation)
+  {lctxTy : Nat → LamSort} {lctxTerm : ∀ n, (lctxTy n).interp lval.ilVal.tyVal}
+  (wf₁ : LamWF lval.ilVal.toLamTyVal ⟨lctxTy, .app (.app (.base (.eq m)) a) b, .base .prop⟩)
+  (H₁ : GLift.down (LamWF.interp lval lctxTy lctxTerm wf₁))
+  (wf₂ : LamWF lval.ilVal.toLamTyVal ⟨lctxTy, .app (.app (.base (.eq n)) b) c, .base .prop⟩)
+  (H₂ : GLift.down (LamWF.interp lval lctxTy lctxTerm wf₂)) :
+  GLift.down (LamWF.interp lval lctxTy lctxTerm (Eq.trans.WF wf₁ wf₂)) :=
+  match wf₁ with
+  | .ofApp argTy₁ wfFn₁ wfB₁ =>
+    match wfFn₁ with
+    | .ofApp argTy₁' wfEq₁ wfA =>
+      match wfEq₁ with
+      | .ofBase HB₁ =>
+        match argTy₁, argTy₁', HB₁ with
+        | _, _, .ofEq _ =>
+          match wf₂ with
+          | .ofApp argTy₂ wfFn₂ wfC =>
+            match wfFn₂ with
+            | .ofApp argTy₂' wfEq₂ wfB₂ =>
+              match wfEq₂ with
+              | .ofBase HB₂ =>
+                match argTy₂, argTy₂', HB₂ with
+                | _, _, .ofEq _ => by
+                  let heq : LamTyVal.eqLamVal _ m = LamTyVal.eqLamVal _ n :=
+                    (LamWF.unique lval.ilVal.toLamTyVal wfB₁ wfB₂).left
+                  dsimp [trans.WF, LamWF.interp, LamBaseWF.interp];
+                  dsimp [trans.WF, LamWF.interp, LamBaseWF.interp] at H₁;
+                  dsimp [trans.WF, LamWF.interp, LamBaseWF.interp] at H₂;
+                  apply EqLift.up;
+                  have H₁' := EqLift.down _ _ _ H₁
+                  have H₂' := EqLift.down _ _ _ H₂
+                  apply eq_of_heq
+                  apply HEq.trans (b:=LamWF.interp lval lctxTy lctxTerm wfA)
+                  case a.h.h₁ => apply LamWF.interp.heq <;> rfl
+                  case a.h.h₂ =>
+                    rw [H₁']; rw [← H₂']; apply LamWF.interp.heq <;> rfl                  
 
 end Auto.Embedding.Lam
